Remove predicative invariants.

pulse/lib/core/PulseCore.BaseHeapSig.fst
@@ -4,250 +4,56 @@ module H2 = PulseCore.Heap2
 open PulseCore.Tags
 open PulseCore.HeapSig
 
-noeq
-type mem : Type u#(a + 1) = {
-    heap: H2.heap u#a;
-    ctr: nat;
-    ghost_ctr: erased nat;
-}
-
-let empty_mem 
-: mem u#a
-= { heap = H2.empty_heap; ctr = 0; ghost_ctr = 0 }
-
-let disjoint_mem (m0 m1: mem)
-: prop
-= H2.disjoint m0.heap m1.heap
-
-let max (i j:nat) : nat = if i >= j then i else j
-let join_mem (m0:mem) (m1:mem { disjoint_mem m0 m1 })
-: mem
-= { heap = H2.join m0.heap m1.heap;
-    ctr = max m0.ctr m1.ctr;
-    ghost_ctr = hide <| max m0.ghost_ctr m1.ghost_ctr }
-
-let sep : separable (mem u#a) = {
-    empty = empty_mem;
-    disjoint = disjoint_mem;
-    join = join_mem;
-    disjoint_sym = (fun m1 m2 -> H2.disjoint_sym m1.heap m2.heap);
-    join_commutative = (fun h0 h1 -> H2.join_commutative h0.heap h1.heap); 
-    disjoint_join = (fun m1 m2 m3 -> H2.disjoint_join m1.heap m2.heap m3.heap);
-    join_associative = (fun h0 h1 h2 -> H2.join_associative h0.heap h1.heap h2.heap);
-    join_empty = (fun m -> H2.join_empty m.heap);
-}
-
-let full_mem_pred m = H2.full_heap_pred m.heap
-
-let is_ghost_action m0 m1 : prop =
-  m0.ctr == m1.ctr /\
-  H2.concrete m0.heap == H2.concrete m1.heap
-
-open FStar.FunctionalExtensionality
-let slprop = p:(mem ^-> prop) { is_affine_mem_prop sep p }
-let interp (p:slprop) : affine_mem_prop sep = p
-  // H2.interp_depends_only_on p;
-  // fun h -> H2.interp p h.heap
-let as_slprop (p:affine_mem_prop sep) : slprop = on _ p
-// = assert (forall m0 m1. H2.disjoint m0 m1 == sep.disjoint m0 m1);
-//   H2.as_slprop p
-
-let lift (p:H2.slprop) : slprop =
+let interp (p:slprop) : affine_mem_prop sep =
   H2.interp_depends_only_on p;
-  as_slprop fun h -> H2.interp p h.heap
+  H2.interp p
+let as_slprop (p:affine_mem_prop sep) : q:slprop{forall h. interp q h <==> p h} =
+  introduce forall (h0 h1: H2.heap u#a). p h0 /\ H2.disjoint h0 h1 ==> p (H2.join h0 h1) with
+    introduce _ ==> _ with _. assert sep.disjoint h0 h1;
+  H2.as_slprop p
 
-[@@erasable]
-noeq
-type uunit : Type u#a = | UU
-let bprop : Type u#a = uunit
-let up (b:bprop) : slprop = lift H2.emp
-let down (p:slprop) : bprop = UU
-let up_down (p:bprop) : Lemma (down (up p) == p) = ()
-
-let emp : slprop = lift H2.emp
 let pure (p:prop) : slprop = as_slprop fun _ -> p
 
-let star' (p1:slprop) (p2:slprop) (m: mem) : prop = 
-  exists m0 m1. 
-    sep.disjoint m0 m1 /\
-    m == sep.join m0 m1 /\
-    interp p1 m0 /\
-    interp p2 m1
-let star'_affine p1 p2 : squash (is_affine_mem_prop sep (star' p1 p2)) =
-  introduce forall m m3. star' p1 p2 m /\ sep.disjoint m m3 ==> star' p1 p2 (sep.join m m3) with
-  introduce _ ==> _ with _. (
-    let m0 = IndefiniteDescription.indefinite_description_ghost _ fun m0 -> exists m1. 
-      sep.disjoint m0 m1 /\ m == sep.join m0 m1 /\ interp p1 m0 /\ interp p2 m1 in
-    let m1 = IndefiniteDescription.indefinite_description_ghost _ fun m1 ->
-      sep.disjoint m0 m1 /\ m == sep.join m0 m1 /\ interp p1 m0 /\ interp p2 m1 in
-    sep.join_commutative m0 m1;
-    sep.join_associative m3 m1 m0;
-    sep.join_commutative m3 (sep.join m0 m1);
-    sep.join_commutative (sep.join m3 m1) m0;
-    sep.join_commutative m3 m1;
-    assert star' p1 p2 (sep.join m0 (sep.join m1 m3))
-  )
-let star (p1:slprop) (p2:slprop) : slprop =
-  star'_affine p1 p2;
-  as_slprop (star' p1 p2)
-let star_equiv (p q:slprop) (m:mem)
-: Lemma (
-    interp (p `star` q) m <==> 
-        (exists m0 m1. 
-          sep.disjoint m0 m1 /\
-          m == sep.join m0 m1 /\
-          interp p m0 /\
-          interp q m1)
-  )
-= ()
+let star_equiv (p q:slprop) (m:mem u#a)
+= assert (forall (m0 m1: mem u#a). sep.disjoint m0 m1 == H2.disjoint m0 m1);
+  introduce interp (p `star` q) m ==>
+      exists m0 m1. sep.disjoint m0 m1 /\ m == sep.join m0 m1 /\ interp p m0 /\ interp q m1 with _.
+    H2.elim_star p q m;
+  introduce forall m0 m1.
+      sep.disjoint m0 m1 /\ m == sep.join m0 m1 /\ interp p m0 /\ interp q m1 ==>
+        interp (p `star` q) m with
+    introduce _ ==> _ with _.
+    H2.intro_star p q m0 m1
 
 let slprop_extensionality (p q:slprop)
 : Lemma ((forall c. interp p c <==> interp q c) ==> p == q)
         [SMTPat (p == q)]
-= introduce (forall c. interp p c <==> interp q c) ==> p == q with _. (
-    introduce forall c. p c == q c with PropositionalExtensionality.apply (p c) (q c);
-    extensionality _ _ p q
-  )
-
-let lift_star (p q: H2.slprop) : squash (lift (p `H2.star` q) == lift p `star` lift q) =  
-  introduce forall c. interp (lift (p `H2.star` q)) c <==> interp (lift p `star` lift q) c with (
-    introduce H2.interp (p `H2.star` q) c.heap ==> interp (lift p `star` lift q) c with _. (
-      H2.elim_star p q c.heap;
-      let h1 = IndefiniteDescription.indefinite_description_ghost _ fun h1 -> exists h2.
-        H2.disjoint h1 h2 /\ c.heap == H2.join h1 h2 /\ H2.interp p h1 /\ H2.interp q h2 in
-      let h2 = IndefiniteDescription.indefinite_description_ghost _ fun h2 ->
-        H2.disjoint h1 h2 /\ c.heap == H2.join h1 h2 /\ H2.interp p h1 /\ H2.interp q h2 in
-      let c1: mem = { c with heap = h1 } in
-      let c2: mem = { c with heap = h2 } in
-      assert sep.disjoint c1 c2
-    );
-    introduce interp (lift p `star` lift q) c ==> H2.interp (p `H2.star` q) c.heap with _. (
-      let c1 = IndefiniteDescription.indefinite_description_ghost _ fun c1 -> exists c2.
-        disjoint_mem c1 c2 /\ c == join_mem c1 c2 /\ interp (lift p) c1 /\ interp (lift q) c2 in
-      let c2 = IndefiniteDescription.indefinite_description_ghost _ fun c2 ->
-        disjoint_mem c1 c2 /\ c == join_mem c1 c2 /\ interp (lift p) c1 /\ interp (lift q) c2 in
-      H2.intro_star p q c1.heap c2.heap
-    )
-  );
-  slprop_extensionality (lift (p `H2.star` q)) (lift p `star` lift q)
+= introduce (forall c. interp p c <==> interp q c) ==> p == q with _.
+  H2.slprop_extensionality p q
 
 let interp_as (p:affine_mem_prop sep)
 : Lemma (forall c. interp (as_slprop p) c == p c)
 = introduce forall c. interp (as_slprop p) c == p c
   with FStar.PropositionalExtensionality.apply (interp (as_slprop p) c) (p c)
 
-let free_above (m:mem u#a) =
-  H2.free_above_addr CONCRETE m.heap m.ctr /\
-  H2.free_above_addr GHOST m.heap m.ghost_ctr
-  // (forall i. i >= m.ghost_ctr ==> None? (H2.select_ghost i m.heap)) /\
-  // (forall i. i >= m.ctr ==> None? (H2.select i m.heap))
-
-let mem_invariant (is:GhostSet.set unit) (m:mem u#a)
-: slprop u#a
-= pure (free_above m)
-
-let dup_pure (p:prop)
-: Lemma (pure p == pure p `star` pure p)
-= FStar.Classical.forall_intro sep.join_empty ;
-  slprop_extensionality (pure p) (pure p `star` pure p)
-
-let iname_of (i:unit) = i
-let inv (i:unit) (p:slprop) = pure False
-let inv_extract (i:unit) (p:slprop u#a) (m:mem u#a)
-: Lemma 
-  (requires interp (inv i p) m)
-  (ensures p == emp)
-= ()
-
-let deq_iref : GhostSet.decide_eq unit = fun x y -> true
-let mem_invariant_equiv (e:GhostSet.set unit) (m:mem u#a) (i:unit) (p:slprop u#a)
-: Lemma 
-  (requires
-    interp (inv i p) m /\
-    ~ (i `GhostSet.mem` e))
-  (ensures
-    mem_invariant e m ==
-    mem_invariant (HeapSig.add deq_iref i e) m `star` p)
-= ()
-
-let dup_inv_equiv (i:unit) (p:slprop)
-: Lemma (inv i p == inv i p `star` inv i p)
-= dup_pure False
-    
 let emp_unit (p:slprop) : Lemma (p == (p `star` emp)) =
   introduce forall (h: _ { interp p h }). interp (p `star` emp) h with (
     let h2 = sep.empty in
     sep.join_empty h;
-    H2.intro_emp h2.heap
+    H2.intro_emp h2;
+    H2.intro_star p emp h h2
+  );
+  introduce forall (h: _ { interp (p `star` emp) h }). interp p h with (
+    star_equiv p emp h
   );
   slprop_extensionality p (p `star` emp)
 
-let star_congruence (p q:slprop)
-: Lemma
-  (requires up (down p) == p /\ up (down q) == q)
-  (ensures up (down (p `star` q)) == p `star` q)
-= emp_unit p; emp_unit q
-
-let update_ghost (m0:mem u#a) (m1:erased (mem u#a) { is_ghost_action m0 m1 })
-: m:mem u#a { m == reveal m1 }
-= { heap = H2.upd_ghost_heap m0.heap m1.heap; ctr = m0.ctr; ghost_ctr = m1.ghost_ctr }
-
 let pure_true_emp () : Lemma (pure True == emp) =
-  introduce forall h. interp (pure True) h <==> interp emp h with H2.intro_emp h.heap;
+  introduce forall h. interp (pure True) h <==> interp emp h with H2.intro_emp h;
   slprop_extensionality (pure True) emp
-let intro_emp (h:mem) : Lemma (interp emp h) = H2.intro_emp h.heap
-let empty_mem_invariant (e:GhostSet.set unit)
-: Lemma (mem_invariant e empty_mem == emp)
-= FStar.Classical.forall_intro H2.free_above_empty;
-  assert (free_above empty_mem);
-  calc (==) {
-    pure (free_above empty_mem);
-  (==) { FStar.PropositionalExtensionality.apply (free_above empty_mem) True }
-    pure True;
-  (==) { pure_true_emp () }
-    emp;
-  }
-let base_heap : heap_sig u#a =
-  {
-    mem;
-    sep;
-    full_mem_pred;
-    is_ghost_action;
-    is_ghost_action_preorder= (fun _ -> ());
-    update_ghost;
-    slprop;
-    interp;
-    as_slprop;
-    interp_as;
-    slprop_extensionality;
-    non_info_slprop = (fun x -> reveal x);
-    bprop;
-    up;
-    down;
-    up_down;
-    emp;
-    pure;
-    star;
-    intro_emp;
-    pure_interp=(fun p c -> ());
-    pure_true_emp;
-    emp_unit;
-    star_equiv;
-    star_congruence;
-    iref = unit;
-    deq_iref;
-    non_info_iref = (fun x -> reveal x);
-    inv;
-    iname_ok = (fun _ _ -> True);
-    dup_inv_equiv;
-    mem_invariant;
-    inv_iname_ok = (fun _ _ _ -> ());
-    mem_invariant_equiv;
-    iref_injective = (fun _ -> false);
-    iref_injectivity = (fun _ _ _ _ _ -> ());
-    empty_mem_invariant
-}
-let join_empty_inverse m0 m1 = H2.join_empty_inverse m0.heap m1.heap
+let intro_emp (h:mem) : Lemma (interp emp h) = H2.intro_emp h
+let pure_interp (p:prop) (c:mem) : Lemma (interp (pure p) c == p) =
+  H2.pure_interp p c; PropositionalExtensionality.apply (interp (pure p) c) p
 let core_ghost_ref_is_null (r:core_ghost_ref) = H2.core_ghost_ref_is_null r
 let core_ghost_ref_as_addr (r:core_ghost_ref)
 : GTot nat
@@ -257,44 +63,13 @@ let addr_as_core_ghost_ref (a:nat)
 = H2.addr_as_core_ghost_ref a
 let core_ghost_ref_as_addr_injective r1 = H2.core_ghost_ref_as_addr_injective r1
 let addr_as_core_ghost_ref_injective a = H2.addr_as_core_ghost_ref_injective a
-let select_ghost i m = H2.select_ghost i m.heap
-let ghost_ctr m = m.ghost_ctr
+let select_ghost i m = H2.select_ghost i m
+let ghost_ctr m = H2.ctr GHOST m
+let ctr m = H2.ctr CONCRETE m
 let empty_mem_props () = 
-  FStar.Classical.forall_intro H2.free_above_empty;
-  FStar.Classical.forall_intro_3 H2.reveal_free_above_addr
-let mem_invariant_interp (ex:inames base_heap) (h0:base_heap.mem) (h1:base_heap.mem)
-: Lemma (base_heap.interp (base_heap.mem_invariant ex h0) h1 ==>
-         free_above_ghost_ctr h0)
-= base_heap.pure_interp (free_above h0) h1;
-  H2.reveal_free_above_addr GHOST h0.heap h0.ghost_ctr
-let inames_ok_trivial (ex:inames base_heap) (h:base_heap.mem)
-: Lemma (inames_ok ex h)
-= ()
-let bump_ghost_ctr (m0:base_heap.mem) (x:erased nat)
-= let ctr = hide (max m0.ghost_ctr x) in
-  let m1 = {m0 with ghost_ctr = ctr} in
-  introduce forall ex c0 c1. 
-    base_heap.interp (base_heap.mem_invariant ex m0) c0 ==>
-    base_heap.interp (base_heap.mem_invariant ex m1) c1
-  with introduce _ ==> _
-  with _ . (
-      base_heap.pure_interp (free_above m0) c0;
-      base_heap.pure_interp (free_above m1) c1;
-      H2.weaken_free_above GHOST m0.heap m0.ghost_ctr m1.ghost_ctr
-  );
-  let m' = { m1 with heap = H2.empty_heap } in
-  H2.join_empty m0.heap;
-  assert m1 == base_heap.sep.join m0 m'; 
-  m1
-
-let pts_to #a #p r c = lift (H2.pts_to #a #p r c)
-let ghost_pts_to meta #a #p r x = lift (H2.ghost_pts_to meta #a #p r x)
-let interp_ghost_pts_to i #meta #a #pcm v h0 = H2.interp_ghost_pts_to i #meta #a #pcm v h0.heap
-let ghost_pts_to_compatible_equiv #meta #a #pcm x v0 v1 =
-  lift_star (H2.ghost_pts_to meta #a #pcm x v0) (H2.ghost_pts_to meta #a #pcm x v1);
-  H2.ghost_pts_to_compatible_equiv #meta #a #pcm x v0 v1;
-  H2.slprop_extensionality (H2.ghost_pts_to meta #a #pcm x v0 `H2.star` H2.ghost_pts_to meta #a #pcm x v1)
-    (H2.ghost_pts_to meta #a #pcm x (op pcm v0 v1))
+  H2.ctr_empty GHOST;
+  H.ctr_prop (H2.ghost empty_mem);
+  FStar.Classical.forall_intro_2 H2.select_ghost_interp
 
 (* Lifting H2 actions *)
 let mg_of_mut (m:Tags.mutability) =
@@ -303,342 +78,161 @@ let mg_of_mut (m:Tags.mutability) =
   | _ -> true
 
 let lower' (frame: slprop) (m: base_heap.mem) (h: H2.heap) : prop =
-  interp frame { m with heap = h }
+  interp frame h
 let lower (frame: slprop) (m: base_heap.mem) : p:H2.slprop { forall h. H2.interp p h <==> lower' frame m h } =
   introduce forall (h0 h1: H2.heap). lower' frame m h0 /\ H2.disjoint h0 h1 ==> lower' frame m (H2.join h0 h1) with
     introduce _ ==> _ with _ . (
-      let m0 = { m with heap = h0 } in
-      let m1 = { m with heap = h1 } in
-      assert sep.disjoint m0 m1
+      assert sep.disjoint h0 h1
     );
   H2.as_slprop (lower' frame m)
 
-let elim_init (e:_) (fp: H2.slprop) (frame:slprop u#a) (m:base_heap.mem)
+let elim_init (fp: H2.slprop) (frame:slprop u#a) (m:base_heap.mem)
 : Lemma 
-  (requires interpret (lift fp `star` frame `star` mem_invariant e m) m)
-  (ensures H2.interp fp m.heap /\ H2.interp (fp `H2.star` lower frame m) m.heap /\ free_above m)
+  (requires interpret (fp `star` frame) m)
+  (ensures H2.interp fp m /\ H2.interp (fp `H2.star` lower frame m) m)
 = ac_lemmas base_heap;
-  HeapSig.destruct_star #base_heap (lift fp `star` frame) (mem_invariant e m) m;
-  HeapSig.destruct_star #base_heap (lift fp) frame m;
-  assert H2.interp fp m.heap;
-  assert free_above m;
+  HeapSig.destruct_star #base_heap fp frame m;
+  assert H2.interp fp m;
+  star_equiv fp frame m;
   let m1 = IndefiniteDescription.indefinite_description_ghost _ fun m1 -> exists m2.
-    disjoint_mem m1 m2 /\ m == join_mem m1 m2 /\ interp (lift fp) m1 /\ interp frame m2 in
+    disjoint_mem m1 m2 /\ m == join_mem m1 m2 /\ interp fp m1 /\ interp frame m2 in
   let m2 = IndefiniteDescription.indefinite_description_ghost _ fun m2 ->
-    disjoint_mem m1 m2 /\ m == join_mem m1 m2 /\ interp (lift fp) m1 /\ interp frame m2 in
+    disjoint_mem m1 m2 /\ m == join_mem m1 m2 /\ interp fp m1 /\ interp frame m2 in
   assert interp frame m2;
-  let m3 = { m with heap = H2.empty_heap } in
-  let m4 = { m with heap = m2.heap } in
-  H2.join_empty m2.heap;
-  assert H2.disjoint m2.heap m3.heap;
+  let m3 = H2.empty_heap in
+  let m4 = m2 in
+  H2.join_empty m2;
+  assert H2.disjoint m2 m3;
   assert disjoint_mem m2 m3;
   assert join_mem m2 m3 == m4;
   assert interp frame m4;
-  assert H2.interp (lower frame m) m4.heap;
+  assert H2.interp (lower frame m) m4;
   assert disjoint_mem m1 m4;
   assert join_mem m1 m4 == m;
-  H2.intro_star fp (lower frame m) m1.heap m4.heap
+  H2.intro_star fp (lower frame m) m1 m4
 
-let intro_fin (e:_) (post: H2.slprop) (frame:slprop) (m:base_heap.mem)
-    (m0: base_heap.mem { m0.ctr <= m.ctr /\ m0.ghost_ctr <= m.ghost_ctr })
+let intro_fin (post: H2.slprop) (frame:slprop) (m:base_heap.mem)
+    (m0: base_heap.mem { ctr m0 <= ctr m /\ ghost_ctr m0 <= ghost_ctr m })
 : Lemma
-  (requires H2.interp (post `H2.star` lower frame m0) m.heap /\ free_above m)
-  (ensures base_heap.interp (lift post `star` frame `star` mem_invariant e m) m)
-= H2.elim_star post (lower frame m0) m.heap;
+  (requires H2.interp (post `H2.star` lower frame m0) m)
+  (ensures base_heap.interp (post `star` frame) m)
+= H2.elim_star post (lower frame m0) m;
   let h1 = IndefiniteDescription.indefinite_description_ghost _ fun h1 -> exists h2.
-    H2.disjoint h1 h2 /\ m.heap == H2.join h1 h2 /\ H2.interp post h1 /\ H2.interp (lower frame m0) h2 in
+    H2.disjoint h1 h2 /\ m == H2.join h1 h2 /\ H2.interp post h1 /\ H2.interp (lower frame m0) h2 in
   let h2 = IndefiniteDescription.indefinite_description_ghost _ fun h2 ->
-    H2.disjoint h1 h2 /\ m.heap == H2.join h1 h2 /\ H2.interp post h1 /\ H2.interp (lower frame m0) h2 in
-  let m1 = { m with heap = h1 } in
-  let m2 = { m with heap = h2 } in
-  assert interp (lift post) m1;
-  let m3 = { m0 with heap = h2 } in
+    H2.disjoint h1 h2 /\ m == H2.join h1 h2 /\ H2.interp post h1 /\ H2.interp (lower frame m0) h2 in
+  let m1 = h1 in
+  let m2 = h2 in
+  assert interp post m1;
+  let m3 = h2 in
   assert interp frame m3;
-  let m4 = { m with heap = H2.empty_heap } in
+  let m4 = H2.empty_heap in
   H2.join_empty h2;
   assert sep.disjoint m3 m4;
   assert join_mem m3 m4 == m2;
   assert interp frame m2;
   assert disjoint_mem m1 m2;
   assert join_mem m1 m2 == m;
-  assert interp (lift post `star` frame) m;
-  ac_lemmas base_heap;
-  HeapSig.intro_pure_frame #base_heap (lift post `star` frame) (free_above m) () m
+  star_equiv post frame m;
+  assert interp (post `star` frame) m;
+  ac_lemmas base_heap
               
 let lift_heap_action
       (#fp:H2.slprop u#a)
       (#a:Type u#b)
       (#fp':a -> H2.slprop u#a)
       (#mut:_)
-      (e:inames base_heap)
       ($f:H2.action #mut #None fp a fp')
-      (#fp_post: a -> slprop u#a { forall x. lift (fp' x) == fp_post x })
-: act:_action_except base_heap a (mg_of_mut mut) e (lift fp) fp_post
-  {
-     mut == IMMUTABLE ==> preserves_inames act  
-  }
-= let act : _action_except base_heap a (mg_of_mut mut) e (lift fp) fp_post =
+      (#fp_post: a -> slprop u#a { forall x. fp' x == fp_post x })
+: _action_except base_heap a (mg_of_mut mut) fp fp_post
+= let act : _action_except base_heap a (mg_of_mut mut) fp fp_post =
     fun frame m0 ->
-      elim_init e fp frame m0;
-      let h0 = m0.heap in
+      elim_init fp frame m0;
+      let h0 = m0 in
       assert H2.interp fp h0;
       let (| x, h1 |) = f h0 in
       assert H2.interp (fp' x) h1;
-      let m1 = {m0 with heap=h1} in
-      assert (H2.interp (fp' x `H2.star` lower frame m0) m1.heap);
+      let m1 = h1 in
+      assert (H2.interp (fp' x `H2.star` lower frame m0) m1);
       assert (H2.action_related_heaps #mut #None h0 h1);
       assert (H2.does_not_allocate CONCRETE h0 h1);
       assert (H2.does_not_allocate GHOST h0 h1);
-      assert (free_above m1);
-      intro_fin e (fp' x) frame m1 m0;
+      intro_fin (fp' x) frame m1 m0;
       assert (maybe_ghost_action base_heap (mg_of_mut mut) m0 m1);
-      assert (inames_ok e m1);
       (x, m1)
   in
-  match mut with
-  | IMMUTABLE ->
-    introduce forall (m0:full_mem base_heap) frame. 
-      interpret (lift fp `base_heap.star` frame `base_heap.star` base_heap.mem_invariant e m0) m0 /\
-      inames_ok e m0
-      ==> ( 
-      let x, m1 = act frame m0 in
-      heaps_preserve_inames m0 m1
-    )
-    with introduce _ ==> _ 
-    with _. ( 
-      let x, m1 = act frame m0 in
-      elim_init e fp frame m0;
-      H2.action_framing f (lower frame m0) m0.heap;
-      assert (H2.action_related_heaps #IMMUTABLE #None m0.heap m1.heap);
-      assert (m0 == m1);
-      assert (heaps_preserve_inames m0 m1)
-    );
-    act
-  | _ -> act
-
-let with_fresh_ghost_counter (#t:Type u#t) (#post:t -> H2.slprop u#a) (e:inames base_heap)
-  (f: (addr:erased nat ->
-        H2.action #ONLY_GHOST #(Some GHOST)
-          #(fun h -> h `H2.free_above_addr GHOST` addr)
-          #(fun h -> h `H2.free_above_addr GHOST` (addr + 1))      
-          H2.emp 
-          t
-          post))
-: ghost_action_except base_heap t e emp (fun x -> lift (post x))
-= fun frame m0 ->
-    elim_init e H2.emp frame m0;
-    let h0 = m0.heap in
-    let (|r, h1|) = f m0.ghost_ctr h0 in
-    let m1 = {m0 with heap=h1; ghost_ctr=m0.ghost_ctr + 1} in
-    intro_fin e (post r) frame m1 m0;
-    r, m1
-
-let ghost_extend_alt
-    (meta:erased bool)
-    (#ex:inames base_heap)
-    (#a:Type u#a)
-    (#pcm:pcm a)
-    (x:erased a{pcm.refine x})
-: ghost_action_except base_heap (ghost_ref a pcm) ex    
-        base_heap.emp 
-        (fun r -> ghost_pts_to meta r x)
-= with_fresh_ghost_counter ex (H2.ghost_extend #meta #a #pcm x)
-
-let ghost_extend_spec_alt
-      (#meta:bool)
-      (#ex:inames base_heap)
-      #a #pcm (x:a { pcm.refine x })
-      (frame:base_heap.slprop)
-      (h:full_mem base_heap { 
-        inames_ok ex h /\
-        interpret (base_heap.emp `base_heap.star`
-                   frame `base_heap.star`
-                   base_heap.mem_invariant ex h) h })      
-: Lemma (
-      let (r, h1) = ghost_extend_alt meta #ex #a #pcm x frame h in
-      single_ghost_allocation meta #a #pcm x r h h1)
-= let act = ghost_extend_alt meta #ex #a #pcm x in
-  let _, m1 = act frame h in
-  elim_init ex H2.emp frame h;
-  H2.ghost_extend_spec #meta #a #pcm x h.ghost_ctr h.heap;
-  HeapSig.destruct_star
-    (base_heap.emp `base_heap.star` frame)
-    (base_heap.mem_invariant ex h) h;
-  assert (interpret (base_heap.mem_invariant ex h) h);
-  mem_invariant_interp ex h h;
-  assert (free_above_ghost_ctr h)
-  
-
-let ghost_extend meta #ex #a #pcm x =
-  let act = ghost_extend_alt meta #ex #a #pcm x in
-  introduce reveal meta == false ==> preserves_inames act
-  with _ . (
-    introduce forall (m0:full_mem base_heap) frame. 
-      interpret (base_heap.emp `base_heap.star` frame `base_heap.star` base_heap.mem_invariant ex m0) m0 /\
-      inames_ok ex m0
-      ==> ( 
-      let r, m1 = act frame m0 in
-      heaps_preserve_inames m0 m1
-    )
-    with introduce _ ==> _
-    with _. (
-      ghost_extend_spec_alt #meta #ex #a #pcm x frame m0;
-      elim_init ex H2.emp frame m0;
-      assert (free_above m0);
-      H2.reveal_free_above_addr GHOST m0.heap m0.ghost_ctr
-    )
-  );
   act
 
-let ghost_extend_spec
-      (#meta:bool)
-      (#ex:inames base_heap)
-      #a #pcm (x:a { pcm.refine x })
-      (frame:base_heap.slprop)
-      (h:full_mem base_heap { 
-        inames_ok ex h /\
-        interpret (base_heap.emp `base_heap.star`
-                   frame `base_heap.star`
-                   base_heap.mem_invariant ex h) h })      
-= ghost_extend_spec_alt #meta #ex #a #pcm x frame h
+let pts_to #a #p r c = H2.pts_to #a #p r c
+let ghost_pts_to #a #p r x = H2.ghost_pts_to #a #p r x
 
-let ghost_read #ex #meta #a #p r x f = lift_heap_action ex (H2.ghost_read #meta #a #p r x f)
-let ghost_write #ex #meta #a #p r x y f = 
-    let act 
-      : ghost_action_except base_heap unit ex
-          (ghost_pts_to meta r x)
-          (fun _ -> ghost_pts_to meta r y)
-      = lift_heap_action ex (H2.ghost_write #meta #a #p r x y f)
-    in
-    introduce reveal meta == false ==> preserves_inames act
-    with _ . (
-      introduce forall (m0:full_mem base_heap) frame. 
-        interpret ((ghost_pts_to meta r x) `base_heap.star` frame `base_heap.star` base_heap.mem_invariant ex m0) m0 /\
-        inames_ok ex m0
-          ==> ( 
-          let x, m1 = act frame m0 in
-          heaps_preserve_inames m0 m1
-        )
-      with introduce _ ==> _ 
-      with _. ( 
-        let _, m1 = act frame m0 in
-        elim_init ex (H2.ghost_pts_to meta #a #p r x) frame m0;
-        H2.ghost_write_modifies #meta #a #p r x y f m0.heap;
-        match (H2.select_ghost (H2.core_ghost_ref_as_addr r) m0.heap) with
-        | None -> ()
-        | Some (H.Ref meta' _ _ _) -> 
-          assert (reveal meta == false);
-          assert (H2.interp (H2.ghost_pts_to meta #a #p r x) m0.heap);
-          interp_ghost_pts_to r #meta #a #p x m0;
-          assert (reveal meta' == false)
-      )
-    );
-    act
-let ghost_share #ex #meta #a #p r x y =
-  lift_star (H2.ghost_pts_to meta #a #p r x) (H2.ghost_pts_to meta #a #p r y);
-  lift_heap_action ex (H2.ghost_share #meta #a #p r x y)
-let ghost_gather #ex #meta #a #p r x y =
-  lift_star (H2.ghost_pts_to meta #a #p r x) (H2.ghost_pts_to meta #a #p r y);
-  lift_heap_action ex (H2.ghost_gather #meta #a #p r x y)
-    #(fun _ -> ghost_pts_to meta r (op p x y))
+let ghost_extend #a #pcm x = fun frame m0 ->
+  let (| y, m1 |) = H2.apply_action (H2.ghost_extend #a #pcm x) frame m0 in
+  y, m1
 
-let with_fresh_counter (#t:Type u#t) (#post:t -> H2.slprop u#a) (e:inames base_heap)
-  (f: (addr:nat ->
-        H2.action #MUTABLE #(Some CONCRETE)
-          #(fun h -> h `H2.free_above_addr CONCRETE` addr)
-          #(fun h -> h `H2.free_above_addr CONCRETE` (addr + 1))      
-          H2.emp 
-          t
-          post))
-: action_except base_heap t e emp (fun x -> lift (post x))
-= fun frame m0 ->
-    elim_init e H2.emp frame m0;
-    let h0 = m0.heap in
-    let (|r, h1|) = f m0.ctr h0 in
-    let m1 = {m0 with heap=h1; ctr=m0.ctr + 1} in
-    intro_fin e (post r) frame m1 m0;
-    r, m1
+let ghost_read #a #p r x f = lift_heap_action (H2.ghost_read #a #p r x f)
+let ghost_write #a #p r x y f = 
+  lift_heap_action (H2.ghost_write #a #p r x y f)
+let ghost_share #a #p r x y =
+  lift_heap_action (H2.ghost_share #a #p r x y)
+let ghost_gather #a #p r x y =
+  lift_heap_action (H2.ghost_gather #a #p r x y)
+    #(fun _ -> ghost_pts_to r (op p x y))
 
-let extend_alt #ex #a #pcm (x:a {pcm.refine x})
-  : action_except base_heap (ref a pcm) ex    
-        base_heap.emp 
-        (fun r -> pts_to r x)
-  = with_fresh_counter ex (H2.extend #a #pcm x)
-let extend #ex #a #pcm (x:a {pcm.refine x})
-: act:action_except base_heap (ref a pcm) ex    
-          base_heap.emp 
-          (fun r -> pts_to r x) {
-            preserves_inames act
-          }
-= let act = extend_alt #ex #a #pcm x in 
-  FStar.Classical.forall_intro_2 H2.select_ghost_interp;
-  introduce forall (m0:full_mem base_heap) frame. 
-      interpret (base_heap.emp `base_heap.star` frame `base_heap.star` base_heap.mem_invariant ex m0) m0 /\
-      inames_ok ex m0
-      ==> ( 
-      let r, m1 = act frame m0 in
-      heaps_preserve_inames m0 m1
-  )
-  with introduce _ ==> _ 
-  with _. ( 
-    let r, m1 = act frame m0 in
-    elim_init ex H2.emp frame m0;
-    H2.extend_modifies #a #pcm x m0.ctr m0.heap
-  );
-  act
+let extend #a #pcm x = fun frame m0 ->
+  let (| y, m1 |) = H2.apply_action (H2.extend #a #pcm x) frame m0 in
+  y, m1
 
-
-let read #ex #a #p r x f = lift_heap_action ex (H2.select_refine #a #p r x f) #(fun v -> pts_to r (f v))
-let write #ex #a #p r x y f = 
-  let act
-    : action_except base_heap unit ex
-        (pts_to r x)
-        (fun _ -> pts_to r y)
-    = lift_heap_action ex (H2.upd_gen_action #a #p r x y f)
-  in
-  FStar.Classical.forall_intro_2 H2.select_ghost_interp;
-  introduce forall (m0:full_mem base_heap) frame. 
-  interpret ((pts_to r x) `base_heap.star` frame `base_heap.star` base_heap.mem_invariant ex m0) m0 /\
-  inames_ok ex m0
-    ==> ( 
-    let x, m1 = act frame m0 in
-    heaps_preserve_inames m0 m1
-  )
-  with introduce _ ==> _ 
-  with _. ( 
-    let _, m1 = act frame m0 in
-    elim_init ex (H2.pts_to #a #p r x) frame m0;
-    H2.upd_gen_modifies #a #p r x y f m0.heap;
-    assert (H2.ghost m0.heap == H2.ghost m1.heap);
-    ()
-  );
-  act
-let share #ex #a #p r x y =
-  lift_star (H2.pts_to #a #p r x) (H2.pts_to #a #p r y);
-  lift_heap_action ex (H2.split_action #a #p r x y)
-let gather #ex #a #p r x y =
-  lift_star (H2.pts_to #a #p r x) (H2.pts_to #a #p r y);
-  lift_heap_action ex (H2.gather_action #a #p r x y)
+let read #a #p r x f = lift_heap_action (H2.select_refine #a #p r x f) #(fun v -> pts_to r (f v))
+let write #a #p r x y f = 
+  lift_heap_action (H2.upd_gen_action #a #p r x y f)
+let share #a #p r x y =
+  lift_heap_action (H2.split_action #a #p r x y)
+let gather #a #p r x y =
+  lift_heap_action (H2.gather_action #a #p r x y)
     #(fun _ -> pts_to r (op p x y))
-let pts_to_not_null_action #ex #a #p r x = lift_heap_action ex (H2.pts_to_not_null_action #a #p r x)
+let pts_to_not_null_action #a #p r x = lift_heap_action (H2.pts_to_not_null_action #a #p r x)
 
-let interp_exists_sem (#a:Type) (p: a -> base_heap.slprop) (m:_)
-: Lemma (interp (exists_ p) m <==> (exists x. interp (p x) m))
-= assert (interp (exists_ p) m == base_heap.interp (exists_ p) m);
-  interp_exists p
+module U = FStar.Universe
+module R = Pulse.Lib.PCM.Raise
 
-let exists_congruence (#a:Type) (witness:a) (p: a -> base_heap.slprop)
-: Lemma 
-  (requires forall x. is_boxable (p x))
-  (ensures is_boxable (exists_ p))
-= introduce forall m. interp (exists_ p) m ==> interp (up (down (exists_ p))) m
-  with introduce _ ==> _
-  with _ . (
-    interp_exists_sem p m
-  );
-  introduce forall m. interp (up (down (exists_ p))) m ==> interp (exists_ p) m
-  with introduce _ ==> _
-  with _ . ( 
-    interp_exists_sem p m 
-  );
-  slprop_extensionality (exists_ p) (up (down (exists_ p)))
+let ghost_pts_to' #a #p r x =
+  H2.ghost_pts_to #(U.raise_t a) #(R.raise p) r (U.raise_val x)
+
+let ghost_extend' #a #p x = fun frame m0 ->
+  ghost_extend #_ #(R.raise p) (U.raise_val (reveal x)) frame m0
+
+let ghost_read' #a #p r x f = fun frame m0 ->
+  let y, m0 = ghost_read #_ #(R.raise p) r (U.raise_val (reveal x)) (R.raise_refine p x f) frame m0 in
+  hide (U.downgrade_val y), m0
+
+let ghost_write' #a #p r x y f = 
+  ghost_write #_ #(R.raise p) r (U.raise_val (reveal x)) (U.raise_val (reveal y)) (R.raise_upd f)
+
+let ghost_share' #a #p r x y =
+  ghost_share #_ #(R.raise p) r (U.raise_val (reveal x)) (U.raise_val (reveal y))
+
+let ghost_gather' #a #p r x y =
+  ghost_gather #_ #(R.raise p) r (U.raise_val (reveal x)) (U.raise_val (reveal y))
+
+let pts_to' #a #p r x =
+  H2.pts_to #(U.raise_t a) #(R.raise p) r (U.raise_val x)
+
+let extend' #a #p x = fun frame m0 ->
+  extend #_ #(R.raise p) (U.raise_val x) frame m0
+
+let read' #a #p r x f = fun frame m0 ->
+  let y, m0 = read #_ #(R.raise p) r (U.raise_val (reveal x)) (R.raise_refine p x f) frame m0 in
+  U.downgrade_val y, m0
+
+let write' #a #p r x y f = 
+  write #_ #(R.raise p) r (U.raise_val (reveal x)) (U.raise_val (reveal y)) (R.raise_upd f)
+
+let share' #a #p r x y =
+  share #_ #(R.raise p) r (U.raise_val (reveal x)) (U.raise_val (reveal y))
+
+let gather' #a #p r x y =
+  gather #_ #(R.raise p) r (U.raise_val (reveal x)) (U.raise_val (reveal y))
+
+let pts_to_not_null_action' #a #p r v =
+  pts_to_not_null_action #_ #(R.raise p) r (U.raise_val (reveal v))
