pulse/lib/core/PulseCore.Heap2.fst
@@ -98,7 +98,7 @@ let emp = as_slprop (fun _ -> True)
 let llift (t:tag) (p:H.slprop) : slprop =
   as_slprop (fun h -> H.of_slprop p (get t h))
 let lift (p:H.slprop) : slprop = llift CONCRETE p
-let pts_to #a #pcm (r:ref a pcm) (v:a) = lift (H.pts_to false #a #pcm r v)
+let pts_to #a #pcm (r:ref a pcm) (v:a) = lift (H.pts_to #a #pcm r v)
 let star p1 p2 =
   as_slprop (fun (h: heap) ->
     exists (h1 h2 : heap).
@@ -166,20 +166,20 @@ let lift_emp : squash (lift H.emp == emp) =
   slprop_extensionality (lift H.emp) emp
 
 let pts_to_compatible #a #pcm (x:ref a pcm) (v0 v1:a) h = 
-  H.pts_to_compatible #false #a #pcm x v0 v1 h.concrete;
-  lift_star CONCRETE (H.pts_to false #a #pcm x v0) (H.pts_to false #a #pcm x v1)
+  H.pts_to_compatible #a #pcm x v0 v1 h.concrete;
+  lift_star CONCRETE (H.pts_to #a #pcm x v0) (H.pts_to #a #pcm x v1)
 
 let pts_to_join #a #pcm (r:ref a pcm) (v1 v2:a) h =
-  H.pts_to_join #false #a #pcm r v1 v2 h.concrete
+  H.pts_to_join #a #pcm r v1 v2 h.concrete
 
 let pts_to_join' #a #pcm r v1 v2 h =
-  H.pts_to_join' #false #a #pcm r v1 v2 h.concrete
+  H.pts_to_join'  #a #pcm r v1 v2 h.concrete
 
 let pts_to_compatible_equiv #a #pcm r v0 v1 =
-  H.pts_to_compatible_equiv #false #a #pcm r v0 v1;
-  lift_star CONCRETE (H.pts_to false #a #pcm r v0) (H.pts_to false #a #pcm r v1)
+  H.pts_to_compatible_equiv #a #pcm r v0 v1;
+  lift_star CONCRETE (H.pts_to #a #pcm r v0) (H.pts_to #a #pcm r v1)
 
-let pts_to_not_null #a #pcm x v m = H.pts_to_not_null #false #a #pcm x v m.concrete
+let pts_to_not_null #a #pcm x v m = H.pts_to_not_null #a #pcm x v m.concrete
 
 let intro_star p q h hq = ()
 let elim_star p q h = ()
@@ -198,19 +198,10 @@ let stronger_star p q r = ()
 let weaken p q r h = ()
 
 let full_heap_pred h = H.full_heap_pred h.concrete /\ H.full_heap_pred h.ghost
-let heap_evolves (h0 h1:full_heap) =
-  H.heap_evolves h0.concrete h1.concrete /\
-  H.heap_evolves h0.ghost h1.ghost
 let select i m = H.select i m.concrete
 let select_ghost i m = H.select i m.ghost
 let select_ghost_interp i m = ()
-let free_above_addr tag h a = H.free_above_addr (get tag h) a
-let free_above_empty (t:tag) : Lemma (free_above_addr t (empty_heap u#a) 0) = 
-  H.free_above_empty ()
-let reveal_free_above_addr tag h a = 
-  H.interp_free_above h.concrete a;
-  H.interp_free_above h.ghost a
-let weaken_free_above tag h a b = H.weaken_free_above (get tag h) a b
+let ctr_empty t = H.ctr_empty ()
 
 (** [sel_v] is a ghost read of the value contained in a heap reference *)
 let sel_v' (#a:Type u#h) (#pcm:pcm a) (r:ref a pcm) (v:erased a) (m:full_hheap (pts_to r v))
@@ -219,30 +210,30 @@ let sel_v' (#a:Type u#h) (#pcm:pcm a) (r:ref a pcm) (v:erased a) (m:full_hheap (
           interp (ptr r) m /\
           True
           }
-  = let v = H.sel_v #false #a #pcm r v m.concrete in
+  = let v = H.sel_v #a #pcm r v m.concrete in
     v
 
 let lower_ptr #a #pcm (r:ref a pcm) (m:full_hheap (ptr r))
-: Lemma (H.interp (H.ptr false #a #pcm r) m.concrete)
-= eliminate exists v. H.interp (H.pts_to false #a #pcm r v) m.concrete
-  returns H.interp (H.ptr false #a #pcm r) m.concrete
-  with _ . ( H.intro_h_exists v (H.pts_to false #a #pcm r) m.concrete )
+: Lemma (H.interp (H.ptr #a #pcm r) m.concrete)
+= eliminate exists v. H.interp (H.pts_to #a #pcm r v) m.concrete
+  returns H.interp (H.ptr #a #pcm r) m.concrete
+  with _ . ( H.intro_h_exists v (H.pts_to #a #pcm r) m.concrete )
 
 let raise_ptr #a #pcm (r:ref a pcm) (m:full_heap)
 : Lemma 
   (requires
-    H.interp (H.ptr false #a #pcm r) m.concrete)
+    H.interp (H.ptr #a #pcm r) m.concrete)
   (ensures
     interp (ptr r) m)
-= H.elim_h_exists (H.pts_to false #a #pcm r) m.concrete;
-  eliminate exists v. H.interp (H.pts_to false #a #pcm r v) m.concrete
+= H.elim_h_exists (H.pts_to #a #pcm r) m.concrete;
+  eliminate exists v. H.interp (H.pts_to #a #pcm r v) m.concrete
   returns interp (ptr #a #pcm r) m
   with _ . ()
 
 (** [sel] is a ghost read of the value contained in a heap reference *)
 let sel (#a:Type u#h) (#pcm:pcm a) (r:ref a pcm) (m:full_hheap (ptr r)) : a =
  lower_ptr r m;
- H.sel #false #a #pcm r m.concrete
+ H.sel #a #pcm r m.concrete
  
 let sel_v (#a:Type u#h) (#pcm:pcm a) (r:ref a pcm) (v:erased a) (m:full_hheap (pts_to r v))
   : v':a{ compatible pcm v v' /\
@@ -250,41 +241,9 @@ let sel_v (#a:Type u#h) (#pcm:pcm a) (r:ref a pcm) (v:erased a) (m:full_hheap (p
           interp (ptr r) m /\
           v' == sel r m
           }
-  = H.sel_v #false #a #pcm r v m.concrete
+  = H.sel_v #a #pcm r v m.concrete
 
-let sel_lemma #a #pcm r m = lower_ptr r m; H.sel_lemma #false #a #pcm r m.concrete
-let heap_evolves_iff (h0 h1:full_heap)
-: Lemma 
-  (ensures
-     heap_evolves h0 h1 <==> (
-      H.heap_evolves h0.concrete h1.concrete /\
-      H.heap_evolves h0.ghost h1.ghost))
-= assert (heap_evolves h0 h1 <==> 
-            (H.heap_evolves h0.concrete h1.concrete /\ H.heap_evolves h0.ghost h1.ghost))
-      by (FStar.Tactics.norm [delta_only [`%heap_evolves]])
-
-
-// let witnessed_ref_stability #a #pcm r fact = 
-//   H.witnessed_ref_stability #a #pcm r fact;
-//   assert (FStar.Preorder.stable (H.witnessed_ref #a #pcm r fact) H.heap_evolves);
-//   introduce forall h0 h1. 
-//     (witnessed_ref r fact h0 /\
-//      heap_evolves h0 h1) ==>
-//     witnessed_ref r fact h1
-//   with (
-//     introduce _ ==> _
-//     with _ . (
-//       assert (interp (ptr r) h0 /\ fact (sel r h0));
-//       lower_ptr r h0;
-//       assert (H.interp (H.ptr #a #pcm r) h0.concrete);
-//       assert (heap_evolves h0 h1);
-//       heap_evolves_iff h0 h1;
-//       assert (H.heap_evolves h0.concrete h1.concrete);
-//       assert (H.witnessed_ref #a #pcm r fact h1.concrete);
-//       raise_ptr r h1;
-//       assert (sel r h1 == H.sel #a #pcm r h1.concrete)
-//     )
-//   )
+let sel_lemma #a #pcm r m = lower_ptr r m; H.sel_lemma #a #pcm r m.concrete
 
 let llift_pred (l:tag) (pre:H.heap -> prop)
   : heap -> prop
@@ -369,23 +328,23 @@ let lift_action
         assert (interp frame h11);
         assert (disjoint h10 h11)
       );
-      heap_evolves_iff h0 h1;
+      // heap_evolves_iff h0 h1;
       assert (action_related_heaps #mut #allocs h0 h1)
     )
   );
   p
 
-let sel_action #a #pcm r v0 = lift_action (H.sel_action #false #a #pcm r v0)
-let select_refine #a #p r x f = lift_action (H.select_refine #false #a #p r x f)
-let upd_gen_action #a #p r x y f = lift_action (H.upd_gen_action #false #a #p r x y f)
-let upd_gen_modifies #a #p r x y f h = H.upd_gen_modifies #false #a #p r x y f h.concrete
-let upd_action #a #p r x y = lift_action (H.upd_action #false #a #p r x y)
-let free_action #a #p r v0 = lift_action (H.free_action #false #a #p r v0)
-let split_action #a #p r v0 v1 = lift_action (H.split_action #false #a #p r v0 v1)
-let gather_action #a #p r v0 v1 = lift_action (H.gather_action #false #a #p r v0 v1)
-let pts_to_not_null_action #a #p r v = lift_action (H.pts_to_not_null_action #false #a #p r v)
-let extend #a #pcm x addr = lift_action (H.extend #false #a #pcm x addr)
-let extend_modifies #a #pcm x addr h = ()
+let sel_action #a #pcm r v0 = lift_action (H.sel_action #a #pcm r v0)
+let select_refine #a #p r x f = lift_action (H.select_refine #a #p r x f)
+let upd_gen_action #a #p r x y f = lift_action (H.upd_gen_action #a #p r x y f)
+let upd_gen_modifies #a #p r x y f h = H.upd_gen_modifies #a #p r x y f h.concrete
+let upd_action #a #p r x y = lift_action (H.upd_action #a #p r x y)
+let free_action #a #p r v0 = lift_action (H.free_action #a #p r v0)
+let split_action #a #p r v0 v1 = lift_action (H.split_action #a #p r v0 v1)
+let gather_action #a #p r v0 v1 = lift_action (H.gather_action #a #p r v0 v1)
+let pts_to_not_null_action #a #p r v = lift_action (H.pts_to_not_null_action #a #p r v)
+let extend #a #pcm x = lift_action (H.extend #a #pcm x)
+let extend_modifies #a #pcm x h = ()
 
 let refined_pre_action (#mut:mutability) (#allocates:option tag)
                        (#[T.exact (`trivial_pre)]pre:heap ->prop)
@@ -446,37 +405,7 @@ let change_slprop (p q:slprop)
     refined_pre_action_as_action g
 
 
-let elim_exists #a p =
-  fun frame h0 ->
-  let w = FStar.IndefiniteDescription.indefinite_description_tot
-    a
-    (fun x -> interp (p x `star` frame) h0) in
-  (| w, h0 |)
-
-let intro_exists #a p x =
-  fun frame h0 ->
-    intro_h_exists (reveal x) p h0;
-    (| (), h0 |)
-
 module U = FStar.Universe    
-
-let lift_exists (#a:_) (p:a -> slprop)
-  : action (h_exists p) unit
-           (fun _a -> h_exists #(U.raise_t a) (U.lift_dom p))
-  = let g : refined_pre_action #IMMUTABLE #no_allocs (h_exists p) unit (fun _a -> h_exists #(U.raise_t a) (U.lift_dom p))
-          = fun h ->
-              introduce forall x h.
-                  interp (p x) h ==>
-                  interp (h_exists (U.lift_dom p)) h
-              with (
-                introduce _ ==> _
-                with _ . (
-                  assert (interp (U.lift_dom p (U.raise_val x)) h)
-                )
-              );
-              (| (), h |)
-    in
-    refined_pre_action_as_action g
 
 let elim_pure (p:prop)
   : action (pure p) (u:unit{p}) (fun _ -> emp)
@@ -497,7 +426,7 @@ let intro_pure (p:prop) (_:squash p)
 let pts_to_evolve (#a:Type u#a) (#pcm:_) (r:ref a pcm) (x y : a) (h:heap)
   : Lemma (requires (interp (pts_to r x) h /\ compatible pcm y x))
           (ensures  (interp (pts_to r y) h))
-  = H.pts_to_evolve #false #a #pcm r x y h.concrete
+  = H.pts_to_evolve #a #pcm r x y h.concrete
 
 let drop p
 = let f
@@ -549,8 +478,7 @@ let lift_erased
 
 let core_ghost_ref = erased H.core_ref
 let core_ghost_ref_eq x y = H.core_ref_eq (reveal x) (reveal y)
-let ghost_pts_to meta #a #p r v = llift GHOST (H.pts_to meta #a #p r v)
-let ghost_free_above_addr h addr = H.free_above_addr h.ghost addr
+let ghost_pts_to #a #p r v = llift GHOST (H.pts_to #a #p r v)
 
 
 let lift_heap_pre_action_ghost
@@ -643,7 +571,7 @@ let lift_action_ghost
         assert (interp frame h11);
         assert (disjoint h10 h11)
       );
-      heap_evolves_iff h0 h1;
+      // heap_evolves_iff h0 h1;
       assert (action_related_heaps #mut #allocs h0 h1)
     )
   );
@@ -733,57 +661,20 @@ let core_ghost_ref_as_addr_injective (c1:core_ghost_ref)
 = H.addr_core_ref_injective_2 c1
 let addr_as_core_ghost_ref_injective (a:nat)
 = H.addr_core_ref_injective a
-let interp_ghost_pts_to i #m #a #p v h = H.interp_pts_to i #m #a #p v h.ghost
-let ghost_pts_to_compatible_equiv #meta #a #pcm r v0 v1 =
-  H.pts_to_compatible_equiv #meta #a #pcm r v0 v1;
-  lift_star GHOST (H.pts_to meta #a #pcm r v0) (H.pts_to meta #a #pcm r v1)
+let interp_ghost_pts_to i #a #p v h = H.interp_pts_to i #a #p v h.ghost
+let ghost_pts_to_compatible_equiv #a #pcm r v0 v1 =
+  H.pts_to_compatible_equiv #a #pcm r v0 v1;
+  lift_star GHOST (H.pts_to #a #pcm r v0) (H.pts_to #a #pcm r v1)
 
 let ghost_extend
-    (#meta:_)
     (#a:Type u#a)
     (#pcm:pcm a)
     (x:erased a{pcm.refine x})
-    (addr:erased nat)
 = lift_erased #_ #(ni_erased H.core_ref)
     (Ghost.hide <|
-      lift_action_ghost (ni_erased H.core_ref) (H.erase_action_result (H.extend #meta #a #pcm x addr)))
-let ghost_extend_spec
-      (#meta:bool)
-      #a #pcm (x:a { pcm.refine x })
-      (addr:nat)
-      (h:full_hheap emp { free_above_addr GHOST h addr })
-= 
-calc (==) {
-    (ghost_extend #meta #a #pcm x addr) h;
-  (==) { _ by (T.trefl()) }
-    lift_erased #(ghost_ref pcm) #(ni_erased H.core_ref) #(Some GHOST)
-       #(fun h -> free_above_addr GHOST h addr)
-       #(fun h -> free_above_addr GHOST h (addr + 1))          
-    (Ghost.hide <|
-      lift_action_ghost (ni_erased H.core_ref)
-       (H.erase_action_result (H.extend #meta #a #pcm x addr))) h;
-  (==) { 
-          lift_erased_sem
-            #(ghost_ref pcm)
-            #(ni_erased H.core_ref)
-            #(Some GHOST)
-            #(fun h -> free_above_addr GHOST h addr)
-            #(fun h -> free_above_addr GHOST h (addr + 1))          
-            (Ghost.hide <|
-              lift_action_ghost (ni_erased H.core_ref)
-              (H.erase_action_result (H.extend #meta #a #pcm x addr)))
-            h
-        }
-    lift_action_ghost (ni_erased H.core_ref)
-       (H.erase_action_result (H.extend #meta #a #pcm x addr)) h;
-}; 
-lift_action_ghost_sem (ni_erased H.core_ref)
-       (H.erase_action_result (H.extend #meta #a #pcm x addr)) h;
-H.erase_action_result_identity (H.extend #meta #a #pcm x addr) h.ghost;
-H.extend_modifies_nothing #meta #a #pcm x addr h.ghost
+      lift_action_ghost (ni_erased H.core_ref) (H.erase_action_result (H.extend #a #pcm x)))
 
 let ghost_read
-    #meta
     (#a:Type)
     (#p:pcm a)
     (r:ghost_ref p)
@@ -793,30 +684,28 @@ let ghost_read
                      FStar.PCM.frame_compatible p x v y})))
 = lift_erased #_ #(ni_erased _) #None
     (Ghost.hide <|
-      lift_action_ghost (ni_erased _) (H.erase_action_result (H.select_refine #meta #a #p r x f)))
+      lift_action_ghost (ni_erased _) (H.erase_action_result (H.select_refine #a #p r x f)))
 
 let ghost_write
-    #meta
     (#a:Type)
     (#p:pcm a)
     (r:ghost_ref p)
     (x y:Ghost.erased a)
     (f:FStar.PCM.frame_preserving_upd p x y)
 : action #ONLY_GHOST #None
-    (ghost_pts_to meta r x)
+    (ghost_pts_to r x)
     unit
-    (fun _ -> ghost_pts_to meta r y)
+    (fun _ -> ghost_pts_to r y)
 = lift_erased #_ #(ni_unit) #None
     (Ghost.hide <|
-      lift_action_ghost ni_unit (H.upd_gen_action #meta #a #p r x y f))
+      lift_action_ghost ni_unit (H.upd_gen_action #a #p r x y f))
 
 let ghost_write_modifies
-      (#meta:bool)
       #a (#p:pcm a)
       (r:ghost_ref p)
       (x y:Ghost.erased a)
       (f:FStar.PCM.frame_preserving_upd p x y)
-      (h:full_hheap (ghost_pts_to meta r x))
+      (h:full_hheap (ghost_pts_to r x))
 : Lemma (
       let (| _, h1 |) = ghost_write r x y f h in
       (forall (a:nat). a <> core_ghost_ref_as_addr r ==> select_ghost a h == select_ghost a h1) /\
@@ -827,45 +716,43 @@ let ghost_write_modifies
     (dsnd (ghost_write r x y f h)).ghost;
   (==) { _ by (T.trefl()) }
     (dsnd (lift_erased #_ #ni_unit #None 
-              (Ghost.hide <| lift_action_ghost ni_unit (H.upd_gen_action #meta #a #p r x y f)) h)).ghost;
-  (==) { lift_erased_sem #_ #ni_unit #None (Ghost.hide <| lift_action_ghost ni_unit (H.upd_gen_action #meta #a #p r x y f)) h }
-    (dsnd  (lift_action_ghost ni_unit (H.upd_gen_action #meta #a #p r x y f) h)).ghost;
-  (==) { lift_action_ghost_sem ni_unit (H.upd_gen_action #meta #a #p r x y f) h }
-    (hide (dsnd (H.upd_gen_action #meta #a #p r x y f h.ghost)));
+              (Ghost.hide <| lift_action_ghost ni_unit (H.upd_gen_action #a #p r x y f)) h)).ghost;
+  (==) { lift_erased_sem #_ #ni_unit #None (Ghost.hide <| lift_action_ghost ni_unit (H.upd_gen_action #a #p r x y f)) h }
+    (dsnd  (lift_action_ghost ni_unit (H.upd_gen_action #a #p r x y f) h)).ghost;
+  (==) { lift_action_ghost_sem ni_unit (H.upd_gen_action #a #p r x y f) h }
+    (hide (dsnd (H.upd_gen_action #a #p r x y f h.ghost)));
   };
-  H.upd_gen_modifies #meta #a #p r x y f h.ghost
+  H.upd_gen_modifies #a #p r x y f h.ghost
 
 
 let ghost_share
-    #meta
     (#a:Type)
     (#pcm:pcm a)
     (r:ghost_ref pcm)
     (v0:FStar.Ghost.erased a)
     (v1:FStar.Ghost.erased a{composable pcm v0 v1})
 : action #IMMUTABLE
-    (ghost_pts_to meta r (v0 `op pcm` v1))
+    (ghost_pts_to r (v0 `op pcm` v1))
     unit
-    (fun _ -> ghost_pts_to meta r v0 `star` ghost_pts_to meta r v1)
+    (fun _ -> ghost_pts_to r v0 `star` ghost_pts_to r v1)
 = lift_erased #_ #(ni_unit) #None
     (Ghost.hide <|
-      lift_action_ghost ni_unit (H.split_action #meta #a #pcm r v0 v1))
+      lift_action_ghost ni_unit (H.split_action #a #pcm r v0 v1))
 
 let ni_squash #a : non_informative (squash a) = fun x -> reveal x
 
 #push-options "--fuel 0 --ifuel 0 --z3rlimit_factor 8 --retry 3" // flaky
 let ghost_gather
-    #meta
     (#a:Type)
     (#pcm:pcm a)
     (r:ghost_ref pcm)
     (v0:FStar.Ghost.erased a)
     (v1:FStar.Ghost.erased a)
 : action #IMMUTABLE 
-    (ghost_pts_to meta r v0 `star` ghost_pts_to meta r v1)
+    (ghost_pts_to r v0 `star` ghost_pts_to r v1)
     (squash (composable pcm v0 v1))
-    (fun _ -> ghost_pts_to meta r (op pcm v0 v1))
+    (fun _ -> ghost_pts_to r (op pcm v0 v1))
 = lift_erased #_ #(ni_squash ) #None
     (Ghost.hide <|
-      lift_action_ghost ni_squash (H.gather_action #meta #a #pcm r v0 v1))
+      lift_action_ghost ni_squash (H.gather_action #a #pcm r v0 v1))
 #pop-options
