pulse/lib/core/PulseCore.HeapSig.fst
@@ -92,14 +92,13 @@ let ac_lemmas (h:heap_sig u#a)
 
 let frame
       (#h:heap_sig u#h)
-      (#opened_invariants:inames h)
       (#maybe_ghost:bool)
       (#a:Type u#a)
       (#pre:h.slprop)
       (#post:a -> GTot h.slprop)
       (frame:h.slprop)
-      ($f:_action_except h a maybe_ghost opened_invariants pre post)
-: _action_except h a maybe_ghost opened_invariants (pre `h.star` frame) (fun x -> post x `h.star` frame)
+      ($f:_action_except h a maybe_ghost pre post)
+: _action_except h a maybe_ghost (pre `h.star` frame) (fun x -> post x `h.star` frame)
 = fun frame' m -> ac_lemmas h; f (frame `h.star` frame') m
 
 let witness_exists_lemma (#h:heap_sig u#h) (#a:Type u#a)
@@ -123,20 +122,6 @@ let witness_exists_lemma (#h:heap_sig u#h) (#a:Type u#a)
   );
   FStar.IndefiniteDescription.indefinite_description_tot a (fun x -> interpret (p x `h.star` frame) m)
 
-let witness_exists 
-      (#h:heap_sig u#h)
-      (#ex:inames h)
-      (#a:Type u#a)
-      (p:a -> GTot h.slprop)
-: ghost_action_except h (erased a) ex
-           (exists_ p)
-           (fun x -> p x)
-= fun frame m ->
-    ac_lemmas h;
-    let x = witness_exists_lemma p (frame `h.star` h.mem_invariant ex m) m in
-    h.is_ghost_action_preorder ();
-    x, m
-
 let intro_exists_lemma
       (#h:heap_sig u#h) (#a:Type u#a)
       (p:a -> GTot h.slprop)
@@ -150,16 +135,15 @@ let intro_exists_lemma
 
 let intro_exists
       (#h:heap_sig u#h)
-      (#opened_invariants:_)
       (#a:Type u#a)
       (p:a -> GTot h.slprop)
       (x:erased a)
-: ghost_action_except h unit opened_invariants
+: ghost_action_except h unit
       (p x)
       (fun _ -> exists_ p)
 = fun frame m ->
     ac_lemmas h;
-    intro_exists_lemma p x (frame `h.star` h.mem_invariant opened_invariants m) m;
+    intro_exists_lemma p x frame m;
     h.is_ghost_action_preorder ();
     (), m
 
@@ -167,16 +151,15 @@ let intro_exists
 module U = FStar.Universe
 let lift_h_exists
       (#h:heap_sig u#h)
-      (#opened_invariants:_)
       (#a:Type u#a)
       (p:a -> GTot h.slprop)
-: ghost_action_except h unit opened_invariants
+: ghost_action_except h unit
     (exists_ p)
     (fun _a -> exists_ #_ #(U.raise_t a) (lift_dom_ghost p))
 = fun frame m ->
     ac_lemmas h;
-    let x = witness_exists_lemma p (frame `h.star` h.mem_invariant opened_invariants m) m in
-    intro_exists_lemma (lift_dom_ghost p) (U.raise_val (reveal x)) (frame `h.star` h.mem_invariant opened_invariants m) m;
+    let x = witness_exists_lemma p frame m in
+    intro_exists_lemma (lift_dom_ghost p) (U.raise_val (reveal x)) frame m;
     h.is_ghost_action_preorder ();
     (), m
 
@@ -191,12 +174,11 @@ let elim_pure_lemma (#h:heap_sig u#h) (p:prop) (frame:h.slprop)
 
 let elim_pure
       (#h:heap_sig u#h)
-      (#opened_invariants:_)
       (p:prop)
-: ghost_action_except h (squash p) opened_invariants (h.pure p) (fun _ -> h.emp)
+: ghost_action_except h (squash p) (h.pure p) (fun _ -> h.emp)
 = fun frame m ->
     ac_lemmas h;
-    elim_pure_lemma p (frame `h.star` h.mem_invariant opened_invariants m) m;
+    elim_pure_lemma p frame m;
     h.is_ghost_action_preorder ();
     (), m
 
@@ -209,13 +191,12 @@ let intro_pure_lemma (#h:heap_sig u#h) (p:prop) (frame:h.slprop) (pf:squash p)
 
 let intro_pure
       (#h:heap_sig u#h)
-      (#opened_invariants:_)
       (p:prop)
       (pf:squash p)
-: ghost_action_except h unit opened_invariants h.emp (fun _ -> h.pure p)
+: ghost_action_except h unit h.emp (fun _ -> h.pure p)
 = fun frame m ->
     ac_lemmas h;
-    intro_pure_lemma p (frame `h.star` h.mem_invariant opened_invariants m) pf m;
+    intro_pure_lemma p frame pf m;
     h.is_ghost_action_preorder ();
     (), m
 
@@ -228,24 +209,22 @@ let drop_lemma (#h:heap_sig u#h) (p:h.slprop) (frame:h.slprop)
 
 let drop 
       (#h:heap_sig u#h)
-      (#opened_invariants:_)
       (p:h.slprop)
-: ghost_action_except h unit opened_invariants p (fun _ -> h.emp)
+: ghost_action_except h unit p (fun _ -> h.emp)
 = fun frame m ->
     ac_lemmas h;
-    drop_lemma p (frame `h.star` h.mem_invariant opened_invariants m) m;
+    drop_lemma p frame m;
     h.is_ghost_action_preorder ();
     (), m
 
 let lift_ghost
       (#h:heap_sig u#h)
-      (#opened_invariants:inames h)
       (#a:Type u#a)
       (#p:h.slprop)
       (#q:a -> GTot h.slprop)
       (ni_a:non_info a)
-      (f:erased (ghost_action_except h a opened_invariants p q))
-: ghost_action_except h a opened_invariants p q
+      (f:erased (ghost_action_except h a p q))
+: ghost_action_except h a p q
 = fun frame m0 ->
     let xm1 : erased (a * full_mem h) = 
         let ff = reveal f in
